made a bunch of changes, including: adding a Choice constructor to finite trees; defining separation classes for fix, fork, and forkJoin; and simplifying / shortening some of the definitions and proofs related to downward-closed sets

theories/TraceMonad.v
@@ -69,6 +69,20 @@ Proof.
 Qed.
 
 
+Instance LR_unit : LR unit := { lr_leq := fun _ _ => True }.
+Proof.
+  constructor; intro; intros; apply I.
+Defined.
+
+Instance LR_pair {A B} `{LR A} `{LR B} : LR (A*B) :=
+  { lr_leq := fun p1 p2 => fst p1 <lr= fst p2 /\ snd p1 <lr= snd p2 }.
+Proof.
+  constructor.
+  - intro p. split; reflexivity.
+  - intros p1 p2 p3 [ R12_l R12_r ] [ R23_l R23_r ].
+    split; etransitivity; eassumption.
+Defined.
+
 Instance LR_arrow {A B} `{LR B} : LR (A -> B) :=
   { lr_leq := fun f g => forall a, f a <lr= g a }.
 Proof.
@@ -84,6 +98,25 @@ Proof.
   - intros P H; assumption.
   - intros P1 P2 P3 impl12 impl23 pf; apply impl23; apply impl12; assumption.
 Defined.
+
+
+(* NOTE: we make this a Definition and *NOT* an Instance so that typeclass
+resolution does not use it everywhere *)
+Definition LR_eq {A} : LR A := {| lr_leq := eq |}.
+
+Class ConstLR (F : Type -> Type) : Type :=
+  { lr_leq_K : forall {A}, LR (F A) }.
+
+Instance LR_ConstLR F `{ConstLR F} A : LR (F A) := lr_leq_K.
+Typeclasses Transparent LR_ConstLR.
+
+(*
+Class LRFunctor (F : Type -> Type) : Type :=
+  { lr_leq_F : forall {A} `{LR A}, LR (F A) }.
+
+Instance LR_LRFunctor F `{LRFunctor F} A `{LR A} : LR (F A) := lr_leq_F.
+Typeclasses Transparent LR_LRFunctor.
+*)
 
 
 (***
@@ -118,6 +151,13 @@ Proof.
   intros a1 a2 R12 a'; simpl; intro in_a'. etransitivity; eassumption.
 Qed.
 
+Program Definition unionDownSet {A} `{LR A} (ds1 ds2: DownSet A) : DownSet A :=
+  {| inDownSet := fun a => inDownSet ds1 a \/ inDownSet ds1 a;
+     downSetClosed := _ |}.
+Next Obligation.
+  destruct H1; [ left | right ]; eapply downSetClosed; eassumption.
+Defined.
+
 Program Definition bindDownSet {A B} `{LR A} `{LR B}
            (dsA: DownSet A) (f: A -> DownSet B) : DownSet B :=
   {| inDownSet := fun b => exists a, inDownSet dsA a /\ inDownSet (f a) b;
@@ -140,162 +180,102 @@ Qed.
 Definition mapDownSet {A B} `{LR A} `{LR B} (f:A -> B) dsA : DownSet B :=
   bindDownSet dsA (fun a => downClose (f a)).
 
-Definition lambdaDownSet {A B} `{LR A} `{LR B}
-           (f: A -> DownSet B) : DownSet (A -> DownSet B) := downClose f.
-
-Lemma Proper_lambdaDownSet {A B} `{LR A} `{LR B} :
-  Proper (lr_leq ==> lr_leq) (lambdaDownSet (A:=A) (B:=B)).
-Proof.
-  intros f1 f2 Rf. apply Proper_downClose. assumption.
-Qed.
-
-Lemma Proper_lambdaDownSet_equiv {A B} `{LR A} `{LR B} :
-  Proper (lr_equiv ==> lr_equiv) (lambdaDownSet (A:=A) (B:=B)).
-Proof.
-  intros f1 f2 Rf. destruct Rf. split; apply Proper_downClose; assumption.
-Qed.
-
-
-Definition applyDownSet {A B} `{LR A} `{LR B}
-           (dsF: DownSet (A -> DownSet B)) (a:A) : DownSet B :=
-  bindDownSet dsF (fun f => f a).
-
-Lemma Proper_applyDownSet A B `{LR A} `{LR B} :
-  Proper (lr_leq ==> lr_leq) (applyDownSet (A:=A) (B:=B)).
-Proof.
-  intros ds1 ds2 Rds a. apply Proper_bindDownSet; [ assumption | ].
-  intro. reflexivity.
-Qed.
-
-Lemma Proper_applyDownSet_equiv A B `{LR A} `{LR B} :
-  Proper (lr_equiv ==> lr_equiv) (applyDownSet (A:=A) (B:=B)).
-Proof.
-  intros ds1 ds2 Rds. destruct Rds.
-  split; intro; apply Proper_applyDownSet; assumption.
-Qed.
-
-
-Lemma downSetBeta {A B} `{LR A} `{LR B} (f: A -> DownSet B) :
-  applyDownSet (lambdaDownSet f) =lr= f.
-Proof.
-  split; simpl; intros.
-  - destruct H1 as [g [Rgf in_ga]]. apply Rgf; assumption.
-  - exists f; split; intros; assumption.
-Qed.
-
-(* NOTE: the reverse direction does not hold, because, e.g., dsF could be the
-union of (downClose f) and (downClose g) where f and g have distinct sets as
-their outputs for a, but (lambdaDownSet (applyDownSet dsF)) would have the union
-of these sets as the output for a. *)
-Lemma downSetEta {A B} `{LR A} `{LR B} (dsF : DownSet (A -> DownSet B)) :
-  dsF <lr= lambdaDownSet (applyDownSet dsF).
-Proof.
-  simpl; intros. exists a. split; assumption.
-Qed.
-
-
-Program Definition fixDownSet {A} `{LR A} (f: DownSet A -> DownSet A) : DownSet A :=
-  {| inDownSet a :=
-       forall ds, f ds <lr= ds -> inDownSet ds a
+(* We define the fixed-point of a set function transformer f as the intersection
+of all f-closed functions g *)
+Program Definition fixDownSet {A B} `{LR A} `{LR B}
+        (f: (A -> DownSet B) -> (A -> DownSet B)) (a:A) : DownSet B :=
+  {| inDownSet b :=
+       forall g, f g <lr= g -> inDownSet (g a) b
   |}.
 Next Obligation.
-  apply (downSetClosed _ _ _ H0). apply H1. apply H2.
+  apply (downSetClosed _ _ _ H1). apply H2. apply H3.
 Defined.
 
-Lemma fixDownSetUnfold {A} `{LR A} (f: DownSet A -> DownSet A)
+(* We then prove this is a fixed-point using the Knaster-Tarski theorem *)
+Lemma fixDownSetUnfold {A B} `{LR A} `{LR B}
+      (f: (A -> DownSet B) -> A -> DownSet B)
       (prp: Proper (lr_leq ==> lr_leq) f) :
-  (fixDownSet (A:=A) f) =lr= f (fixDownSet f).
+  (fixDownSet (A:=A) (B:=B) f) =lr= f (fixDownSet f).
 Proof.
   assert (f (fixDownSet f) <lr= fixDownSet f).
-  - intros a in_a ds ds_f_closed.
-    assert (f (fixDownSet f) <lr= ds).
+  - intros a b in_b g g_f_closed.
+    assert (f (fixDownSet f) <lr= g).
     + etransitivity; try eassumption. apply prp.
-      intros a' in_a'. apply in_a'. assumption.
-    + apply H0; assumption.
-  - split; [ | apply H0 ].
-    simpl; intros; apply (H1 _ (prp _ _ H0)).
+      intros a' b' in_b'. apply in_b'. assumption.
+    + apply H1; assumption.
+  - split; [ | apply H1 ].
+    simpl; intros; apply (H2 _ (prp _ _ H1)).
 Qed.
 
-(* FIXME: come up with a better name for this! *)
-Definition fixDownSetFun {A B} `{LR A} `{LR B}
-           (f: (A -> DownSet B) -> (A -> DownSet B))
-  : A -> DownSet B :=
-  applyDownSet (fixDownSet (fun ds => lambdaDownSet (f (applyDownSet ds)))).
-
-Lemma fixDownSetFunUnfold {A B} `{LR A} `{LR B}
-      (f: (A -> DownSet B) -> (A -> DownSet B))
-      (prp: Proper (lr_leq ==> lr_leq) f) :
-  fixDownSetFun f =lr= f (fixDownSetFun f).
+Instance Proper_fixDownSet {A B} `{LR A} `{LR B} :
+  Proper (lr_leq ==> lr_leq) (fixDownSet (A:=A) (B:=B)).
 Proof.
-  unfold fixDownSetFun.
-  etransitivity.
-  - apply Proper_applyDownSet_equiv. apply fixDownSetUnfold.
-    intros ds1 ds2 Rds. apply Proper_lambdaDownSet. apply prp.
-    apply Proper_applyDownSet. assumption.
-  - rewrite downSetBeta. reflexivity.
-Qed.
+  admit. (* FIXME HERE *)
+Admitted.
 
 
-(***
- *** Finite Computation Trees
- ***)
+(* We can convert a function from A to sets of B to a set of functions from A to
+B, by taking the set of all functions that are in f pointwise *)
+Program Definition lambdaDownSet {A B} `{LR B}
+        (f: A -> DownSet B) : DownSet (A -> B) :=
+  {| inDownSet := fun g => forall a, inDownSet (f a) (g a); |}.
+Next Obligation.
+  eapply downSetClosed; [ apply H0 | apply H1 ].
+Defined.
 
-Inductive FinCompTree St A : Type :=
-| TreeStuck
-| TreeLeaf (s:St) (a:A)
-| TreeNode (s:St) (step: St -> FinCompTree St A)
-.
-
-Arguments TreeStuck {St A}.
-Arguments TreeLeaf {St A} s a.
-Arguments TreeNode {St A} s step.
-
-Fixpoint extendsFCT {St A} (tree1 tree2 : FinCompTree St A) : Prop :=
-  match (tree1, tree2) with
-  | (TreeStuck, _) => True
-  | (TreeLeaf s1 a1, TreeLeaf s2 a2) => s1 = s2 /\ a1 = a2
-  | (TreeNode s1 step1, TreeNode s2 step2) =>
-    s1 = s2 /\ forall s, extendsFCT (step1 s) (step2 s)
-  | _ => False
-  end.
-
-Instance PreOrder_extendsFCT {St A} : PreOrder (@extendsFCT St A).
+Instance Proper_lambdaDownSet {A B} `{LR B} :
+  Proper (lr_leq ==> lr_leq) (lambdaDownSet (A:=A) (B:=B)).
 Proof.
-  constructor.
-  - intros tree; induction tree; simpl; auto.
-  - intros tree1; induction tree1 as [ | | s a IH ];
-      intros tree2 tree3;
-      destruct tree2; destruct tree3; simpl; intros R12 R23;
-        try auto; try contradiction.
-    + destruct R12 as [ Rs12 Ra12 ]; destruct R23 as [ Rs23 Ra23 ].
-      split; [ rewrite Rs12; rewrite Rs23 | rewrite Ra12; rewrite Ra23 ];
-        reflexivity.
-    + destruct R12 as [ Rs12 Ra12 ]; destruct R23 as [ Rs23 Ra23 ].
-      split; [ rewrite Rs12; rewrite Rs23; reflexivity | ].
-      intro. apply (IH _ _ _ (Ra12 _) (Ra23 _)).
+  intros f1 f2 R12 g in_g a. apply R12. apply in_g.
 Qed.
 
-Instance LR_FinCompTree {St A} : LR (FinCompTree St A) :=
-  { lr_leq := extendsFCT; lr_PreOrder := _ }.
+Definition applyDownSet {A B} `{LR B}
+           (dsF: DownSet (A -> B)) (a:A) : DownSet B :=
+  mapDownSet (fun f => f a) dsF.
+
+(* NOTE: applyDownSet is not Proper in its A argument unless we somehow build
+Proper functions from the functions in dsF... *)
+Instance Proper_applyDownSet {A B} `{LR B} :
+  Proper (lr_leq ==> eq ==> lr_leq) (applyDownSet (A:=A) (B:=B)).
+Proof.
+  intros ds1 ds2 Rds a1 a2 eq_a b in_b. destruct in_b as [ g [ in_g1 in_g2 ]].
+  rewrite <- eq_a.
+  exists g. split.
+  - apply Rds; assumption.
+  - assumption.
+Qed.
+
+(* NOTE: the reverse only holds when f a is non-empty for all a; i.e., when
+   there is some function g such that inDownSet (f a) (g a) for all a *)
+Lemma downSetBeta {A B} `{LR B} (f: A -> DownSet B) :
+  applyDownSet (lambdaDownSet f) <lr= f.
+Proof.
+  simpl; intros a b in_b.
+  destruct in_b as [ g [ in_ga Rbg ]].
+  eapply downSetClosed; [ apply Rbg | apply in_ga ].
+Qed.
 
 
 (***
  *** Transition Monads
  ***)
 
-Class MonadTraceOps M St : Type :=
+Class MonadTraceOps M St `{ConstLR M} : Type :=
   {
+    (* Monadic return and bind *)
     returnM : forall {A}, A -> M A;
     bindM : forall {A B}, M A -> (A -> M B) -> M B;
+
+    (* State operations *)
     getM : M St;
     putM : St -> M unit;
+
+    (* Threading operations *)
     yieldM : M unit;
   }.
 
-Class MonadTrace M St `{MonadTraceOps M St} : Type :=
+Class MonadTrace M St `{MonadTraceOps M St} : Prop :=
   {
-    Monad_LR {A} :> LR (M A);
-
     Proper_bindM {A B} :
       Proper (lr_leq ==> lr_leq ==> lr_leq) (bindM (A:=A) (B:=B));
 
@@ -306,23 +286,119 @@ Class MonadTrace M St `{MonadTraceOps M St} : Type :=
     monad_assoc {A B C} m (f: A -> M B) (g: B -> M C) :
       bindM (bindM m f) g =lr= bindM m (fun x => bindM (f x) g);
 
-    (* FIXME HERE: write the state monad laws! *)
+    (* FIXME: write the state and threading monad laws! *)
   }.
+
+Class MonadForkJoinOps M : Type :=
+  {
+    forkJoinM : forall {A B}, M A -> M B -> M (A*B)%type;
+  }.
+
+Class MonadForkJoin M `{ConstLR M} `{MonadForkJoinOps M} : Prop :=
+  {
+    Proper_forkJoinM {A B} :
+      Proper (lr_leq ==> lr_leq ==> lr_leq) (forkJoinM (A:=A) (B:=B));
+    (* FIXME: write forkJoin laws...? *)
+  }.
+
+Class MonadForkOps M : Type :=
+  {
+    forkM : M unit -> M unit;
+  }.
+
+Class MonadFork M `{ConstLR M} `{MonadForkOps M} : Prop :=
+  {
+    Proper_forkM : Proper (lr_leq ==> lr_leq) (forkM (M:=M));
+    (* FIXME: write fork laws...? *)
+  }.
+
+Class MonadFixOps M : Type :=
+  {
+    fixM : forall {A B} `{LR A} `{LR B},
+      ((A -> M B) -> (A -> M B)) -> A -> M B;
+  }.
+
+Class MonadFix M `{ConstLR M} `{MonadFixOps M} : Prop :=
+  {
+    Proper_fixM {A B} `{LR A} `{LR B} :>
+      Proper (lr_leq ==> lr_leq) (fixM (A:=A) (B:=B));
+    fixM_correct :
+      forall {A B} `{LR A} `{LR B} (f: (A -> M B) -> (A -> M B)),
+        Proper (lr_leq ==> lr_leq) f ->
+        fixM f =lr= f (fixM f)
+  }.
+
+
+(***
+ *** Finite Computation Trees
+ ***)
+
+Inductive FinCompTree St A : Type :=
+| CompStuck
+| CompDone (s:St) (a:A)
+| CompStep (s:St) (step: St -> FinCompTree St A)
+| CompChoice : FinCompTree St A -> FinCompTree St A -> FinCompTree St A
+.
+
+Arguments CompStuck {St A}.
+Arguments CompDone {St A} s a.
+Arguments CompStep {St A} s step.
+Arguments CompChoice {St A} tree1 tree2.
+
+Fixpoint extendsFCT {St A} (tree1 tree2 : FinCompTree St A) : Prop :=
+  match (tree1, tree2) with
+  | (CompStuck, _) => True
+  | (CompDone s1 a1, CompDone s2 a2) => s1 = s2 /\ a1 = a2
+  | (CompStep s1 step1, CompStep s2 step2) =>
+    s1 = s2 /\ forall s, extendsFCT (step1 s) (step2 s)
+  | (CompChoice t1 t1', CompChoice t2 t2') =>
+    extendsFCT t1 t2 /\ extendsFCT t1' t2'
+  | _ => False
+  end.
+
+Instance PreOrder_extendsFCT {St A} : PreOrder (@extendsFCT St A).
+Proof.
+  constructor.
+  - intros tree; induction tree; simpl; auto.
+  - intros tree1; induction tree1 as [ | | s a IH | ];
+      intros tree2 tree3;
+      destruct tree2; destruct tree3; simpl; intros R12 R23;
+        try auto; try contradiction.
+    + destruct R12 as [ Rs12 Ra12 ]; destruct R23 as [ Rs23 Ra23 ].
+      split; [ rewrite Rs12; rewrite Rs23 | rewrite Ra12; rewrite Ra23 ];
+        reflexivity.
+    + destruct R12 as [ Rs12 Ra12 ]; destruct R23 as [ Rs23 Ra23 ].
+      split; [ rewrite Rs12; rewrite Rs23; reflexivity | ].
+      intro. apply (IH _ _ _ (Ra12 _) (Ra23 _)).
+    + destruct R12 as [ R12_1 R12_2 ]; destruct R23 as [ R23_1 R23_2 ].
+      split; [ eapply IHtree1_1 | eapply IHtree1_2 ]; eassumption.
+Qed.
+
+Instance LR_FinCompTree {St A} : LR (FinCompTree St A) :=
+  { lr_leq := extendsFCT; lr_PreOrder := _ }.
 
 
 (***
  *** The Finite Trace Monad
  ***)
 
-Definition FinTraceMonad St A := St -> FinCompTree St A.
+(* The finite trace monad *)
+Definition FinTraceM St A := St -> FinCompTree St A.
 
+(* Typeclass resolution mostly finds this instance for us *)
+Instance ConstLR_FinTraceM St : ConstLR (FinTraceM St) :=
+  Build_ConstLR _ _.
+
+(* Bind on a computation tree, applying f after the computation terminates *)
 Fixpoint bindFinTree {St A B} (fct: FinCompTree St A)
-         (f : A -> FinTraceMonad St B) : FinCompTree St B :=
+         (f : A -> FinTraceM St B) : FinCompTree St B :=
   match fct with
-  | TreeStuck => TreeStuck
-  | TreeLeaf s a => f a s
-  | TreeNode s step =>
-    TreeNode s (fun s' => bindFinTree (step s') f)
+  | CompStuck => CompStuck
+  | CompDone s a => f a s
+  | CompStep s step =>
+    CompStep s (fun s' => bindFinTree (step s') f)
+  | CompChoice fct1 fct2 =>
+    CompChoice (bindFinTree fct1 f) (bindFinTree fct2 f)
   end.
 
 Instance Proper_bindFinTree St A B :
@@ -331,16 +407,66 @@ Proof.
   admit. (* FIXME HERE *)
 Admitted.
 
-Instance MonadTraceOps_FinTraceMonad St : MonadTraceOps (FinTraceMonad St) St :=
+(* Build the computation that nondeterministically (via CompChoice) applies the
+function f on some CompStep in fct *)
+Fixpoint applyAtSomeStepFCT {St A B}
+         (f: (St -> FinCompTree St A) -> (St -> FinCompTree St B))
+         (fct: FinCompTree St A) : FinCompTree St B :=
+  match fct with
+  | CompStuck => CompStuck
+  | CompDone s a => f (fun s' => CompDone s' a) s
+  | CompStep s step =>
+    CompChoice
+      (CompStep s (f step))
+      (CompStep s (fun s' => applyAtSomeStepFCT f (step s')))
+  | CompChoice fct1 fct2 =>
+    CompChoice (applyAtSomeStepFCT f fct1) (applyAtSomeStepFCT f fct2)
+  end.
+
+Fixpoint forkJoinFCT {St A B} (fct: FinCompTree St A)
+         (mb: St -> FinCompTree St B) : FinCompTree St (A*B) :=
+  match fct with
+  | CompStuck => CompStuck
+  | CompDone s a =>
+    bindFinTree (mb s) (fun b s' => CompDone s' (a,b))
+  | CompStep s step =>
+    CompChoice
+      (CompStep s (fun s' => forkJoinFCT (step s') mb))
+      (CompStep
+         s
+         (fun s' =>
+            applyAtSomeStepFCT
+              (fun mb' s' => forkJoinFCT (step s') mb')
+              (mb s)))
+  | CompChoice fct1 fct2 =>
+    CompChoice (forkJoinFCT fct1 mb) (forkJoinFCT fct2 mb)
+  end.
+
+Instance MonadTraceOps_FinTraceM St : MonadTraceOps (FinTraceM St) St :=
   {|
-    returnM A a := fun s => TreeLeaf s a;
+    returnM A a := fun s => CompDone s a;
     bindM A B m f := fun s => bindFinTree (m s) f;
-    getM := fun s => TreeLeaf s s;
-    putM s := fun _ => TreeLeaf s tt;
-    yieldM := fun s => TreeNode s (fun s => TreeLeaf s tt)
+    getM := fun s => CompDone s s;
+    putM s := fun _ => CompDone s tt;
+    yieldM := fun s => CompStep s (fun s => CompDone s tt);
   |}.
 
-Instance MonadTrace_FinTraceMonad St : MonadTrace (FinTraceMonad St) St.
+Instance MonadTrace_FinTraceM St : MonadTrace (FinTraceM St) St.
+Proof.
+  admit. (* FIXME HERE *)
+Admitted.
+
+Instance MonadForkJoinOps_FinTraceM St : MonadForkJoinOps (FinTraceM St) :=
+  {|
+    forkJoinM :=
+      fun A B m1 m2 s =>
+        CompChoice
+          (forkJoinFCT (m1 s) m2)
+          (bindFinTree (forkJoinFCT (m2 s) m1)
+                       (fun (ba:B*A) s' => CompDone s' (snd ba, fst ba)))
+  |}.
+
+Instance MonadForkJoin_FinTraceM St : MonadForkJoin (FinTraceM St).
 Proof.
   admit. (* FIXME HERE *)
 Admitted.
@@ -350,49 +476,92 @@ Admitted.
  *** The Trace Monad
  ***)
 
-Definition CompTree St A := DownSet (FinCompTree St A).
+Definition TraceM St A := DownSet (FinTraceM St A).
 
-Program Definition TreeNodeF {St A} (s:St)
-           (step: St -> CompTree St A) : CompTree St A :=
-  {| inDownSet fct :=
-         exists step',
-           fct <lr= TreeNode s step' /\
-           forall s', inDownSet (step s) (step' s')
-  |}.
-Next Obligation.
-  destruct a1; simpl in H1; try contradiction;
-    destruct a2; simpl in H; try contradiction; simpl.
-  - exists H0; split; [ apply I | assumption ].
-  - exists H0; split; [ apply I | assumption ].
-  - destruct H as [ eq10 R10 ]; destruct H1 as [ eq0_ R0_ ].
-    exists H0; split; [ split | ]; intros.
-    + etransitivity; eassumption.
-    + etransitivity; [ apply R10 | apply R0_ ].
-    + apply H2.
-Defined.
+Instance ConstLR_TraceM St : ConstLR (TraceM St) := Build_ConstLR _ _.
 
-Definition TraceMonad St A := St -> CompTree St A.
-
-Fixpoint bindFinTreeTM {St A B} (fct: FinCompTree St A)
-        (f: A -> TraceMonad St B) : CompTree St B :=
-  match fct with
-  | TreeStuck => downClose TreeStuck
-  | TreeLeaf s a => f a s
-  | TreeNode s step =>
-    TreeNodeF s (fun s' => bindFinTreeTM (step s') f)
-  end.
-
-Instance MonadTraceOps_TraceMonad St : MonadTraceOps (TraceMonad St) St :=
+Instance MonadTraceOps_TraceM St : MonadTraceOps (TraceM St) St :=
   {|
-    returnM A a s := downClose (returnM a s);
-    bindM A B m f s :=
-      bindDownSet (m s) (fun fct => bindFinTreeTM fct f);
-    getM s := downClose (getM s);
-    putM s s' := downClose (putM s s');
-    yieldM s := downClose (yieldM s);
+    returnM A a := downClose (returnM a);
+    bindM A B m f :=
+      bindDownSet m (fun fin_m =>
+                       mapDownSet (bindM fin_m) (lambdaDownSet f));
+    getM := downClose getM;
+    putM s := downClose (putM s);
+    yieldM := downClose yieldM
   |}.
 
-Instance MonadTrace_TraceMonad St : MonadTrace (TraceMonad St) St.
+Instance MonadTrace_TraceM St : MonadTrace (TraceM St) St.
+Proof.
+  admit. (* FIXME HERE *)
+Admitted.
+
+Instance MonadForkJoinOps_TraceM St : MonadForkJoinOps (TraceM St) :=
+  {|
+    forkJoinM A B m1 m2 :=
+      bindDownSet m1 (fun (fin_m1: FinTraceM St A) =>
+                        mapDownSet (forkJoinM fin_m1) m2)
+  |}.
+
+Instance MonadForkJoin_TraceM St : MonadForkJoin (TraceM St).
+Proof.
+  admit. (* FIXME HERE *)
+Admitted.
+
+Instance MonadFixOps_TraceM St : MonadFixOps (TraceM St) :=
+  {|
+    fixM A B lrA lrB f := fixDownSet f
+  |}.
+
+Instance MonadFix_TraceM St : MonadFix (TraceM St).
+Proof.
+  admit. (* FIXME HERE *)
+Admitted.
+
+
+(***
+ *** The Continuation-Trace Monad
+ ***)
+
+Definition ContTraceM St A := (A -> TraceM St unit) -> TraceM St unit.
+
+Instance ConstLR_ContTraceM St : ConstLR (ContTraceM St) := Build_ConstLR _ _.
+
+Instance MonadTraceOps_ContTraceM St : MonadTraceOps (ContTraceM St) St :=
+  {|
+    returnM A a := fun k => k a;
+    bindM A B m f := fun k => m (fun x => f x k);
+    getM := fun k => bindM getM k;
+    putM s := fun k => bindM (putM s) k;
+    yieldM := fun k => bindM yieldM k;
+  |}.
+
+Instance MonadTrace_ContTraceM St : MonadTrace (ContTraceM St) St.
+Proof.
+  admit.
+Admitted.
+
+Instance MonadFixOps_ContTraceM St : MonadFixOps (ContTraceM St) :=
+  {|
+    fixM A B lrA lrB f a k :=
+      fixDownSet (fun g ak => f (fun a' k' => g (a', k')) (fst ak) (snd ak)) (a,k)
+  |}.
+
+Instance MonadFix_ContTraceM St : MonadFix (ContTraceM St).
+Proof.
+  admit.
+Admitted.
+
+Instance MonadForkOps_ContTraceM St : MonadForkOps (ContTraceM St) :=
+  {|
+    forkM :=
+      fun (m: ContTraceM St unit) =>
+        (fun k =>
+           bindM (forkJoinM (m returnM) (k tt)) (fun _ => returnM tt))
+        : ContTraceM St unit
+  |}.
+
+Instance MonadFork_ContTraceM St : MonadFork (ContTraceM St).
 Proof.
   admit.
 Admitted.
@@ -404,12 +573,12 @@ Admitted.
 
 Definition stepsTo1 {St A} `{LR A} : relation (St * TraceMonad St A) :=
   fun stm1 stm2 =>
-    TreeNodeF (fst stm2) (snd stm2) <lr= (snd stm1) (fst stm1).
+    CompStepF (fst stm2) (snd stm2) <lr= (snd stm1) (fst stm1).
 
 Definition stepsTo {St A} `{LR A} := clos_trans _ (stepsTo1 (St:=St) (A:=A)).
 
 Definition evalsTo1 {St A} `{LR A} (stm : St * TraceMonad St A) (res : St * A) :=
-  inDownSet ((snd stm) (fst stm)) (TreeLeaf (fst res) (snd res)).
+  inDownSet ((snd stm) (fst stm)) (CompDone (fst res) (snd res)).
 
 Definition evalsTo {St A} `{LR A} (stm : St * TraceMonad St A) (res : St * A) :=
   exists2 stm', stepsTo stm stm' & evalsTo1 stm' res.
